Phi_System/Phi_Types.thy
@@ -708,6 +708,7 @@ declare [[\<phi>trace_reasoning = 0]]
        and Separation_Monoid
        and \<open>Functionality T P \<Longrightarrow> Functionality (\<big_ast>\<^sup>\<phi> I T) (\<lambda>x. (\<forall>i \<in> I. P (x i)))\<close>
        and Semimodule_Identity
+       and Semimodule_Zero
 
 term \<open>Functionality T P \<Longrightarrow> Functionality (\<big_ast>\<^sup>\<phi> I T) (\<lambda>x. (\<forall>i \<in> I. P (x i))) \<close>
 
